proofs/hol_light/x86_64/proofs/mlkem_reduce.ml
@@ -290,6 +290,22 @@ let mlkem_reduce_mc =
 let mlkem_reduce_tmc = define_trimmed "mlkem_reduce_tmc" mlkem_reduce_mc;;
 let mlkem_reduce_TMC_EXEC = X86_MK_CORE_EXEC_RULE mlkem_reduce_tmc;;
 
+let LENGTH_MLKEM_REDUCE_TMC =
+  REWRITE_CONV[mlkem_reduce_tmc] `LENGTH mlkem_reduce_tmc`
+  |> CONV_RULE(RAND_CONV LENGTH_CONV);;
+
+let MLKEM_REDUCE_POSTAMBLE_LENGTH = new_definition
+  `MLKEM_REDUCE_POSTAMBLE_LENGTH = 1`;;
+
+let MLKEM_REDUCE_CORE_END = new_definition
+  `MLKEM_REDUCE_CORE_END = LENGTH mlkem_reduce_tmc - MLKEM_REDUCE_POSTAMBLE_LENGTH`;;
+
+let LENGTH_SIMPLIFY_CONV =
+  REWRITE_CONV[LENGTH_MLKEM_REDUCE_TMC;
+              MLKEM_REDUCE_CORE_END;
+              MLKEM_REDUCE_POSTAMBLE_LENGTH] THENC
+  NUM_REDUCE_CONV THENC REWRITE_CONV [ADD_0];;
+
 (* Enable simplification of word_subwords by default.
    Nedded to prevent the symbolic simulation to explode
    as we add more instructions. *)
@@ -333,7 +349,7 @@ let helper_lemma = prove
 let MLKEM_REDUCE_CORRECT = prove(
   `!a x pc.
         aligned 32 a /\
-        nonoverlapping (word pc, 854) (a, 512)
+        nonoverlapping (word pc, LENGTH mlkem_reduce_tmc) (a, 512)
         ==> ensures x86
              (\s. bytes_loaded s (word pc) (BUTLAST mlkem_reduce_tmc) /\
                   read RIP s = word pc /\
@@ -341,7 +357,7 @@ let MLKEM_REDUCE_CORRECT = prove(
                   !i. i < 256
                       ==> read(memory :> bytes16(word_add a (word(2 * i)))) s =
                           x i)
-             (\s. read RIP s = word (pc + 854) /\
+             (\s. read RIP s = word (pc + MLKEM_REDUCE_CORE_END) /\
                   !i. i < 256
                       ==> ival(read(memory :> bytes16
                                  (word_add a (word(2 * i)))) s) =
@@ -353,6 +369,7 @@ let MLKEM_REDUCE_CORRECT = prove(
               MAYCHANGE [ZMM0; ZMM1; ZMM2; ZMM3; ZMM4; ZMM5;
                          ZMM6; ZMM7; ZMM8; ZMM9; ZMM12])`,
 
+  CONV_TAC LENGTH_SIMPLIFY_CONV THEN
   REWRITE_TAC[fst mlkem_reduce_TMC_EXEC] THEN
   REPEAT STRIP_TAC THEN
   REWRITE_TAC[C_ARGUMENTS] THEN
@@ -419,7 +436,9 @@ let MLKEM_REDUCE_NOIBT_SUBROUTINE_CORRECT = prove
                           ival(x i) rem &3329)
               (MAYCHANGE [RSP] ,, MAYCHANGE_REGS_AND_FLAGS_PERMITTED_BY_ABI ,,
                MAYCHANGE [memory :> bytes(a, 512)])`,
-  X86_PROMOTE_RETURN_NOSTACK_TAC mlkem_reduce_tmc MLKEM_REDUCE_CORRECT);;
+  CONV_TAC LENGTH_SIMPLIFY_CONV THEN
+  X86_PROMOTE_RETURN_NOSTACK_TAC mlkem_reduce_tmc
+    (CONV_RULE LENGTH_SIMPLIFY_CONV MLKEM_REDUCE_CORRECT));;
 
 (* NOTE: This must be kept in sync with the CBMC specification
  * in mlkem/src/native/x86_64/src/arith_native_x86_64.h *)
@@ -469,7 +488,7 @@ let full_spec = ONCE_DEPTH_CONV MEMACCESS_INBOUNDS_DEDUP_CONV full_spec |> concl
 let MLKEM_REDUCE_SAFE = time prove
  (`exists f_events.
        forall e a pc.
-           aligned 32 a /\ nonoverlapping (word pc,854) (a,512)
+           aligned 32 a /\ nonoverlapping (word pc,LENGTH mlkem_reduce_tmc) (a,512)
            ==> ensures x86
                (\s.
                     bytes_loaded s (word pc) (BUTLAST mlkem_reduce_tmc) /\
@@ -477,12 +496,13 @@ let MLKEM_REDUCE_SAFE = time prove
                     C_ARGUMENTS [a] s /\
                     read events s = e)
                (\s.
-                    read RIP s = word (pc + 854) /\
+                    read RIP s = word (pc + MLKEM_REDUCE_CORE_END) /\
                     (exists e2.
                          read events s = APPEND e2 e /\
                          e2 = f_events a pc /\
                          memaccess_inbounds e2 [a,512] [a,512]))
                (\s s'. T)`,
-  ASSERT_CONCL_TAC full_spec THEN
+  CONV_TAC LENGTH_SIMPLIFY_CONV THEN
+  ASSERT_CONCL_TAC (rhs(concl(LENGTH_SIMPLIFY_CONV full_spec))) THEN
   PROVE_SAFETY_SPEC_TAC ~public_vars:public_vars mlkem_reduce_TMC_EXEC);;
 
